formal/inference/Code_Generation.thy
@@ -108,7 +108,29 @@ code_pred satisfies_trace.
 
 declare ListMem_iff [code]
 
-export_code iterative_learn finfun_apply infer_types heuristic_1 iefsm2dot efsm2dot GExp.conjoin naive_score null_generator null_modifier nondeterministic learn in Scala
+primrec ran :: "nat \<Rightarrow> nat set" where
+  "ran 0 = {0}" |
+  "ran (Suc n) = insert (Suc n) (ran n)"
+
+lemma "i \<in> ran n = (i \<le> n)"
+proof(induct n)
+  case 0
+  then show ?case by simp
+next
+  case (Suc n)
+  then show ?case
+    by auto
+qed
+
+definition is_generalisation_of :: "transition \<Rightarrow> transition \<Rightarrow> iEFSM \<Rightarrow> bool" where
+  "is_generalisation_of t' t e = (\<exists>i \<in> (ran (max_input e)).
+                                  \<exists>r \<in> (ran (max_reg e)).
+                                  \<exists>to \<in> fset (S e).
+                                  \<exists>from \<in> fset (S e).
+                                  \<exists>uid \<in> fset (uids e).  i < max_reg e \<and> from |\<in>| S e \<and>  t' = remove_guard_add_update t i r \<and> (uid, (from, to), t') |\<in>| e)"
+
+
+export_code is_generalisation_of iterative_learn finfun_apply infer_types heuristic_1 iefsm2dot efsm2dot GExp.conjoin naive_score null_generator null_modifier nondeterministic learn in Scala
   (* module_name "Inference" *)
   file "../../inference-tool/src/main/scala/inference/Inference.scala"
 
